centaur/bitops:
  - Slightly improve efficiency of rotate-left and rotate-right.
  - Add a rule about signed-byte-p of (+ 1 (lognot x)), which may sometimes
    be useful when two's complementing numbers.
  - Update extra-defs.lisp to use define for better documentation, and minor
    efficiency tweaking using type declarations.

centaur/clex:

  - Minor bugfix to defcharset
  - Minor package tweaks in support of future changes

centaur/bridge:

  - Add DEFINE to BRIDGE package, in support of future changes

xdoc:

  - Switch to use str::rchars-to-string where appropriate
  - Switch to use oslib::catpath instead of acl2::extend-pathname

centaur/satlink:

  - Tweak satlink package so that satlink is imported, for better
    looking xdoc manual

centaur/vl:

  - Modernize dupeinst-check

books/centaur/bitops/extra-defs.lisp
@@ -21,288 +21,313 @@
 (in-package "ACL2")
 (local (include-book "ihsext-basics"))
 (local (include-book "arithmetic/top" :dir :system))
+(include-book "cutil/define" :dir :system)
 (include-book "centaur/misc/arith-equivs" :dir :system)
 (include-book "ihs/logops-definitions" :dir :system)
-(include-book "xdoc/top" :dir :system)
+(local (include-book "signed-byte-p"))
 
-; extra-defs.lisp
-;
-; These are some functions I wanted when writing specs for integer and
-; packed-integer instructions.
+(defsection extra-defs
+  :parents (bitops)
+  :short "Additional bitwise operations."
+  :long "<p>This is just an ad-hoc collection of low-level bit operations,
+mostly developed in support of specifying various integer and packed-integer
+instructions.</p>")
 
 (local (in-theory (enable* arith-equiv-forwarding)))
 
-(defun nth-slice2 (n x)
-  "Extract the Nth 2-bit slice of the integer X."
-  (declare (xargs :guard (and (natp n)
-                              (integerp x))))
+
+(define nth-slice2 ((n natp)
+                    (x integerp))
+  :returns (slice natp :rule-classes :type-prescription)
+  :parents (extra-defs)
+  :short "Extract the @('n')th 2-bit slice of the integer @('x')."
+  :long "<p>We leave this enabled; we would usually not expect to try to reason
+about it.</p>"
+  :enabled t
+  :inline t
   (mbe :logic
        (logand (ash (ifix x) (* (nfix n) -2)) (1- (expt 2 2)))
        :exec
-       (logand (ash x (* n -2)) #x3)))
+       (the (unsigned-byte 2)
+         (logand (ash x (the (integer * 0) (* n -2))) #x3)))
+  ///
+  (defcong nat-equiv equal (nth-slice2 n x) 1)
+  (defcong int-equiv equal (nth-slice2 n x) 2)
+  (defthm unsigned-byte-p-2-of-nth-slice2
+    (unsigned-byte-p 2 (nth-slice2 n x))))
 
-(defcong nat-equiv equal (nth-slice2 n x) 1)
-(defcong int-equiv equal (nth-slice2 n x) 2)
 
-(defun nth-slice8 (n x)
-  "Extract the Nth 8-bit slice of the integer X."
-  (declare (xargs :guard (and (natp n)
-                              (integerp x))))
+(define nth-slice8 ((n natp)
+                    (x integerp))
+  :returns (slice natp :rule-classes :type-prescription)
+  :parents (extra-defs)
+  :short "Extract the @('n')th 8-bit slice of the integer @('x')."
+  :long "<p>We leave this enabled; we would usually not expect to try to reason
+about it.</p>"
+  :enabled t
+  :inline t
   (mbe :logic
        (logand (ash (ifix x) (* (nfix n) -8)) (1- (expt 2 8)))
        :exec
-       (logand (ash x (* n -8)) #xFF)))
+       (the (unsigned-byte 8)
+         (logand (ash x (* n -8)) #xFF)))
+  ///
+  (defcong nat-equiv equal (nth-slice8 n x) 1)
+  (defcong int-equiv equal (nth-slice8 n x) 2)
+  (defthm unsigned-byte-p-8-of-nth-slice8
+    (unsigned-byte-p 8 (nth-slice8 n x))))
 
-(defcong nat-equiv equal (nth-slice8 n x) 1)
-(defcong int-equiv equal (nth-slice8 n x) 2)
 
-(defun nth-slice16 (n x)
-  "Extract the Nth 16-bit slice of the integer X."
-  (declare (xargs :guard (and (natp n)
-                              (integerp x))))
+(define nth-slice16 ((n natp)
+                     (x integerp))
+  :returns (slice natp :rule-classes :type-prescription)
+  :parents (extra-defs)
+  :short "Extract the @('n')th 16-bit slice of the integer @('x')."
+  :long "<p>We leave this enabled; we would usually not expect to try to reason
+about it.</p>"
+  :enabled t
+  :inline t
   (mbe :logic
        (logand (ash (ifix x) (* (nfix n) -16)) (1- (expt 2 16)))
        :exec
-       (logand (ash x (* n -16)) #xFFFF)))
+       (the (unsigned-byte 16)
+         (logand (ash x (* n -16)) #xFFFF)))
+  ///
+  (defcong nat-equiv equal (nth-slice16 n x) 1)
+  (defcong int-equiv equal (nth-slice16 n x) 2)
+  (defthm unsigned-byte-p-16-of-nth-slice16
+    (unsigned-byte-p 16 (nth-slice16 n x))))
 
-(defcong nat-equiv equal (nth-slice16 n x) 1)
-(defcong int-equiv equal (nth-slice16 n x) 2)
 
-
-(defun nth-slice32 (n x)
-  "Extract the Nth 32-bit slice of the integer X."
-  (declare (xargs :guard (and (natp n)
-                              (integerp x))))
+(define nth-slice32 ((n natp)
+                     (x integerp))
+  :returns (slice natp :rule-classes :type-prescription)
+  :parents (extra-defs)
+  :short "Extract the @('n')th 32-bit slice of the integer @('x')."
+  :long "<p>We leave this enabled; we would usually not expect to try to reason
+about it.</p>"
+  :enabled t
+  :inline t
   (mbe :logic
        (logand (ash (ifix x) (* (nfix n) -32)) (1- (expt 2 32)))
        :exec
-       (logand (ash x (* n -32)) #ux_FFFF_FFFF)))
+       (the (unsigned-byte 32)
+         (logand (ash x (* n -32)) #ux_FFFF_FFFF)))
+  ///
+  (defcong nat-equiv equal (nth-slice32 n x) 1)
+  (defcong int-equiv equal (nth-slice32 n x) 2)
+  (defthm unsigned-byte-p-32-of-nth-slice32
+    (unsigned-byte-p 32 (nth-slice32 n x))))
 
-(defcong nat-equiv equal (nth-slice32 n x) 1)
-(defcong int-equiv equal (nth-slice32 n x) 2)
 
-
-(defun nth-slice64 (n x)
-  "Extract the Nth 64-bit slice of the integer X."
-  (declare (xargs :guard (and (natp n)
-                              (integerp x))))
+(define nth-slice64 ((n natp)
+                     (x integerp))
+  :returns (slice natp :rule-classes :type-prescription)
+  :parents (extra-defs)
+  :short "Extract the @('n')th 32-bit slice of the integer @('x')."
+  :long "<p>We leave this enabled; we would usually not expect to try to reason
+about it.</p>"
+  :enabled t
+  :inline t
   (mbe :logic
        (logand (ash (ifix x) (* (nfix n) -64)) (1- (expt 2 64)))
        :exec
-       (logand (ash x (* n -64)) #ux_FFFF_FFFF_FFFF_FFFF)))
-
-(defcong nat-equiv equal (nth-slice64 n x) 1)
-(defcong int-equiv equal (nth-slice64 n x) 2)
-
-
-
-(defthm natp-of-nth-slice2
-  (natp (nth-slice2 n x))
-  :rule-classes :type-prescription)
-
-(defthm natp-of-nth-slice8
-  (natp (nth-slice8 n x))
-  :rule-classes :type-prescription)
-
-(defthm natp-of-nth-slice16
-  (natp (nth-slice16 n x))
-  :rule-classes :type-prescription)
-
-(defthm natp-of-nth-slice32
-  (natp (nth-slice32 n x))
-  :rule-classes :type-prescription)
-
-(defthm natp-of-nth-slice64
-  (natp (nth-slice64 n x))
-  :rule-classes :type-prescription)
+       (the (unsigned-byte 64)
+         (logand (ash x (* n -64)) #ux_FFFF_FFFF_FFFF_FFFF)))
+  ///
+  (defcong nat-equiv equal (nth-slice64 n x) 1)
+  (defcong int-equiv equal (nth-slice64 n x) 2)
+  (defthm unsigned-byte-p-64-of-nth-slice64
+    (unsigned-byte-p 64 (nth-slice64 n x))))
 
 
-
-
-(defun negate-slice8 (x)
-  "X is an 8-bit natural.  Treat it as a signed, 8-bit value.  Compute the
-two's complement negation of X, and return it as an 8-bit natural.  For
-instance, (negate-slice8 3) = 253."
-  (declare (xargs :guard (natp x)))
+(define negate-slice8 ((x :type (unsigned-byte 8)))
+  :returns (~x natp :rule-classes :type-prescription)
+  :parents (extra-defs)
+  :short "@(call negate-slice8) computes the 8-bit two's complement negation of
+@('x') and returns it as an 8-bit natural."
+  :long "<p>For example, @('(negate-slice8 3) = 253').</p>
+<p>We leave this enabled; we would usually not expect to try to reason about
+it.</p>"
+  :inline t
+  :enabled t
   (mbe :logic
        (logand (+ 1 (lognot (nfix x))) (1- (expt 2 8)))
        :exec
-       (logand (+ 1 (lognot x)) #xFF)))
+       (the (unsigned-byte 8)
+         (logand (the (signed-byte 9)
+                   (+ 1 (the (signed-byte 9) (lognot x))))
+                 #xFF)))
+  ///
+  (defcong nat-equiv equal (negate-slice8 x) 1)
+  (defthm unsigned-byte-p-8-of-negate-slice8
+    (unsigned-byte-p 8 (negate-slice8 x))))
 
-(defcong nat-equiv equal (negate-slice8 x) 1)
 
-
-(defun negate-slice16 (x)
-  "X is a 16-bit natural.  Treat it as a signed, 16-bit value.  Compute the
-   two's complement negation of X and return it as a 16-bit natural."
-  (declare (xargs :guard (natp x)))
+(define negate-slice16 ((x :type (unsigned-byte 16)))
+  :returns (~x natp :rule-classes :type-prescription)
+  :parents (extra-defs)
+  :short "@(call negate-slice16) computes the 16-bit two's complement negation
+of @('x') and returns it as an 16-bit natural."
+  :long "<p>We leave this enabled; we would usually not expect to try to reason
+about it.</p>"
+  :inline t
+  :enabled t
   (mbe :logic
        (logand (+ 1 (lognot (nfix x))) (1- (expt 2 16)))
        :exec
-       (logand (+ 1 (lognot x)) #xFFFF)))
+       (the (unsigned-byte 16)
+         (logand (the (signed-byte 17)
+                   (+ 1 (the (signed-byte 17) (lognot x))))
+                 #xFFFF)))
+  ///
+  (defcong nat-equiv equal (negate-slice16 x) 1)
+  (defthm unsigned-byte-p-16-of-negate-slice16
+    (unsigned-byte-p 16 (negate-slice16 x))))
 
-(defcong nat-equiv equal (negate-slice16 x) 1)
 
-(defun negate-slice32 (x)
-  "X is a 32-bit natural.  Treat it as a signed, 32-bit value.  Compute the
-two's complement negation of X and return it as a 32-bit natural."
-  (declare (xargs :guard (natp x)))
+(define negate-slice32 ((x :type (unsigned-byte 32)))
+  :returns (~x natp :rule-classes :type-prescription)
+  :parents (extra-defs)
+  :short "@(call negate-slice32) computes the 32-bit two's complement negation
+of @('x') and returns it as an 32-bit natural."
+  :long "<p>We leave this enabled; we would usually not expect to try to reason
+about it.</p>"
+  :inline t
+  :enabled t
   (mbe :logic
        (logand (+ 1 (lognot (nfix x))) (1- (expt 2 32)))
        :exec
-       (logand (+ 1 (lognot x)) #ux_FFFF_FFFF)))
+       (the (unsigned-byte 32)
+         (logand (the (signed-byte 33)
+                   (+ 1 (the (signed-byte 33) (lognot x))))
+                 #ux_FFFF_FFFF)))
+  ///
+  (defcong nat-equiv equal (negate-slice32 x) 1)
+  (defthm unsigned-byte-p-32-of-negate-slice32
+    (unsigned-byte-p 32 (negate-slice32 x))))
 
-(defcong nat-equiv equal (negate-slice32 x) 1)
 
-(defun negate-slice64 (x)
-  "X is a 64-bit natural.  Treat it as a signed, 64-bit value.  Compute the
-two's complement negation of X and return it as a 64-bit natural."
-  (declare (xargs :guard (natp x)))
+(define negate-slice64 ((x :type (unsigned-byte 64)))
+  :returns (~x natp :rule-classes :type-prescription)
+  :parents (extra-defs)
+  :short "@(call negate-slice64) computes the 64-bit two's complement negation
+of @('x') and returns it as an 64-bit natural."
+  :long "<p>We leave this enabled; we would usually not expect to try to reason
+about it.</p>"
+  :enabled t
   (mbe :logic
        (logand (+ 1 (lognot (nfix x))) (1- (expt 2 64)))
        :exec
-       (logand (+ 1 (lognot x)) #ux_FFFF_FFFF_FFFF_FFFF)))
-
-(defcong nat-equiv equal (negate-slice64 x) 1)
-
-(defthm natp-of-negate-slice8
-  (natp (negate-slice8 x))
-  :rule-classes :type-prescription)
-
-(defthm natp-of-negate-slice16
-  (natp (negate-slice16 x))
-  :rule-classes :type-prescription)
-
-(defthm natp-of-negate-slice32
-  (natp (negate-slice32 x))
-  :rule-classes :type-prescription)
-
-(defthm natp-of-negate-slice64
-  (natp (negate-slice64 x))
-  :rule-classes :type-prescription)
-
-
-; BOZO consider extending ihsext-basics with stuff about expt-2.
-(local (defthm posp-expt-2
-         (<= 0 (expt 2 width))
-         :rule-classes ((:rewrite)
-                        (:linear)
-                        (:type-prescription))
-         :hints(("Goal" :in-theory (enable expt)))))
-
-(local (defthm integerp-expt-2
-         (implies (<= 0 width)
-                  (integerp (expt 2 width)))
-         :rule-classes ((:rewrite)
-                        (:type-prescription))
-         :hints(("Goal" :in-theory (enable expt)))))
+       (the (unsigned-byte 64)
+         (logand (the (signed-byte 65)
+                   (+ 1 (the (signed-byte 65) (lognot x))))
+                 #ux_FFFF_FFFF_FFFF_FFFF)))
+  ///
+  (defcong nat-equiv equal (negate-slice64 x) 1)
+  (defthm unsigned-byte-p-64-of-negate-slice64
+    (unsigned-byte-p 64 (negate-slice64 x))))
 
 
 
-(defund abs-diff (a b) ;; Disabled since abs-diff-correct is nicer for reasoning.
+(define abs-diff ((a integerp)
+                  (b integerp))
+  :returns (ans natp :rule-classes :type-prescription)
+  :parents (extra-defs)
+  :short "@(call abs-diff) is just @('(abs (- (ifix a) (ifix b)))'), but
+optimized for @(see gl)."
 
-  "(ABS-DIFF A B) is provably equal to (ABS (- (IFIX A) (IFIX B))).
+  :long "<p>@('abs-diff') is similar to @('(abs (- a b))') but has better
+performance for symbolic simulations with GL: it decides whether the
+subtraction will be necessary by looking at the arguments, which tend to be
+simple and perhaps nicely interleaved, instead of by looking at the result,
+which tend to be complex since they are the combined arguments.</p>
 
-ABS-DIFF performs better than (ABS (- A B)) for symbolic simulation with GL: it
-decides whether the subtraction will be necessary by looking at the arguments,
-which tend to be simple and nicely interleaved, instead of by looking at the
-result, which tend to be complex since they are the combined arguments.
+<p>For an @('aig-cert-mode') proof of the 64-bit @('PSADBW') instruction, using
+@('abs-diff') instead of @('(abs (- a b))') reduced the proof time from 56.2
+seconds to 37.44 seconds.</p>
 
-For an AIG-CERT-MODE proof of the 64-bit PSADBW instruction, using ABS-DIFF
-instead of (ABS (- A B)) reduced the proof time from 56.2 seconds to 37.44
-seconds."
-    (declare (xargs :guard (and (integerp a)
-                                (integerp b))))
-    (mbe :logic
-         ;; Don't be tempted to change the :logic definition to (abs (- (ifix
-         ;; a) (ifix b))).  GL uses :logic definitions!
-         (let ((a (ifix a))
-               (b (ifix b)))
-           (if (<= b a)
-               (- a b)
-             (- b a)))
-         :exec
+<p>We disable this function, but we leave enabled the following theorem:</p>
+
+@(thm abs-diff-correct)
+
+<p>We therefore would not expect to ever need to reason about @('abs-diff')
+directly.</p>"
+
+  (mbe :logic
+       ;; Don't be tempted to change the :logic definition to (abs (- (ifix a)
+       ;; (ifix b))).  GL uses :logic definitions!
+       (let ((a (ifix a))
+             (b (ifix b)))
          (if (<= b a)
              (- a b)
-           (- b a))))
-
-(defthm abs-diff-correct
-  (equal (abs-diff a b)
-         (abs (- (ifix a) (ifix b))))
-  :hints(("Goal" :in-theory (enable abs-diff))))
-
-(defthm natp-of-abs-diff
-  (natp (abs-diff a b))
-  :rule-classes :type-prescription)
-
+           (- b a)))
+       :exec
+       (if (<= b a)
+           (- a b)
+         (- b a)))
+  ///
+  (defthm abs-diff-correct
+    (equal (abs-diff a b)
+           (abs (- (ifix a) (ifix b))))))
 
 
-(defun setbit (n x)
-  "Set X[n] := 1"
-  (declare (xargs :guard (and (natp n)
-                              (integerp x))))
+(define setbit ((n natp     "Bit position to set to 1.")
+                (x integerp "Starting value."))
+  :returns (ans integerp :rule-classes :type-prescription)
+  :parents (extra-defs)
+  :short "Set X[n] := 1"
+  :enabled t
   (let ((n (lnfix n))
         (x (lifix x)))
-    (logior (ash 1 n) x)))
-
-(defcong nat-equiv equal (setbit n x) 1)
-(defcong int-equiv equal (setbit n x) 2)
-
-(defthm integerp-of-setbit
-  (integerp (setbit n x))
-  :rule-classes :type-prescription)
+    (logior (ash 1 n) x))
+  ///
+  (defcong nat-equiv equal (setbit n x) 1)
+  (defcong int-equiv equal (setbit n x) 2))
 
 
-(defun clearbit (n x)
-  "Set X[n] := 0"
-  (declare (xargs :guard (and (natp n)
-                              (integerp x))))
+(define clearbit ((n natp     "Bit position to clear to 0.")
+                  (x integerp "Starting value."))
+  :returns (ans integerp :rule-classes :type-prescription)
+  :parents (extra-defs)
+  :short "Set X[n] := 0"
+  :enabled t
   (let ((n (lnfix n))
         (x (lifix x)))
-    (logand (lognot (ash 1 n)) x)))
-
-(defcong nat-equiv equal (clearbit n x) 1)
-(defcong int-equiv equal (clearbit n x) 2)
-
-(defthm integerp-of-clearbit
-  (integerp (clearbit n x))
-  :rule-classes :type-prescription)
+    (logand (lognot (ash 1 n)) x))
+  ///
+  (defcong nat-equiv equal (clearbit n x) 1)
+  (defcong int-equiv equal (clearbit n x) 2))
 
 
-(defun copybit (n from to)
-  "Set To[n] := From[n]"
-  (declare (xargs :guard (and (natp n)
-                              (integerp from)
-                              (integerp to))))
+(define copybit ((n    natp     "Bit position to copy.")
+                 (from integerp)
+                 (to   integerp))
+  :returns (ans integerp :rule-classes :type-prescription)
+  :parents (extra-defs)
+  :short "Set To[n] := From[n]"
+  :enabled t
   (if (logbitp n from)
       (setbit n to)
-    (clearbit n to)))
-
-(defcong nat-equiv equal (copybit n x y) 1)
-(defcong int-equiv equal (copybit n x y) 2)
-(defcong int-equiv equal (copybit n x y) 3)
-
-
-(defthm integerp-of-copybit
-  (integerp (copybit n from to))
-  :rule-classes :type-prescription)
+    (clearbit n to))
+  ///
+  (defcong nat-equiv equal (copybit n x y) 1)
+  (defcong int-equiv equal (copybit n x y) 2)
+  (defcong int-equiv equal (copybit n x y) 3))
 
 
-(defun notbit (n x)
-  "Set X[n] := ~X[n]"
-  (declare (xargs :guard (and (natp n)
-                              (integerp x))))
+(define notbit ((n natp     "Bit position to negate.")
+                (x integerp "Starting value."))
+  :returns (ans integerp :rule-classes :type-prescription)
+  :parents (extra-defs)
+  :short "Set X[n] := ~X[n]"
+  :enabled t
   (if (logbitp n x)
       (clearbit n x)
-    (setbit n x)))
-
-(defcong nat-equiv equal (notbit n x) 1)
-(defcong int-equiv equal (notbit n x) 2)
-
-(defthm integerp-of-notbit
-  (integerp (notbit n x))
-  :rule-classes :type-prescription)
-
+    (setbit n x))
+  ///
+  (defcong nat-equiv equal (notbit n x) 1)
+  (defcong int-equiv equal (notbit n x) 2))
 
 
 (local
@@ -311,94 +336,99 @@ seconds."
             (< (logtail 1 src) src))
    :hints(("Goal" :in-theory (e/d (logtail**))))))
 
-(defund bitscan-fwd (src)
-  "(BITSCAN-FWD SRC) returns the bit position of the least significant bit in
-SRC that is set, or 0 when SRC is zero (and hence has no such bit)."
-  (declare (xargs :guard (natp src)
-                  :measure (nfix src)))
+(define bitscan-fwd ((src natp))
+  :returns (position natp :rule-classes :type-prescription)
+  :parents (extra-defs)
+  :short "@(call bitscan-fwd) returns the bit position of the least significant
+bit in @('src') that is set, or 0 when @('src') is zero (and hence has no such
+bit)."
+  :long "<p>Examples:</p>
+@({
+     (bitscan-fwd #b1001) = 0
+     (bitscan-fwd #b1010) = 1
+     (bitscan-fwd #b1100) = 2
+     (bitscan-fwd #b1000) = 3
+})"
   (cond ((zp src)         0)
         ((logbitp 0 src)  0)
-        (t                (+ 1 (bitscan-fwd (ash src -1))))))
+        (t                (+ 1 (bitscan-fwd (ash src -1)))))
+  ///
+  (local (defthmd bitscan-fwd-examples
+           ;; This is just to try to "validate the spec" by showing it produces the
+           ;; values we want for some examples.
+           (and
+            ;; Some basic examples...
+            (equal (bitscan-fwd #ub_0000_0000_0001) 0)
+            (equal (bitscan-fwd #ub_0000_0000_0010) 1)
+            (equal (bitscan-fwd #ub_0000_0000_0100) 2)
+            (equal (bitscan-fwd #ub_0000_0000_1000) 3)
+            (equal (bitscan-fwd #ub_0000_0001_0000) 4)
+            (equal (bitscan-fwd #ub_0000_0010_0000) 5)
+            (equal (bitscan-fwd #ub_0000_0100_0000) 6)
+            ;; Same examples, but with upper bits changed to 1s...
+            (equal (bitscan-fwd #ub_0100_0101_0001) 0)
+            (equal (bitscan-fwd #ub_0110_0110_1010) 1)
+            (equal (bitscan-fwd #ub_1010_0101_0100) 2)
+            (equal (bitscan-fwd #ub_1010_1110_1000) 3)
+            (equal (bitscan-fwd #ub_1111_1111_0000) 4)
+            (equal (bitscan-fwd #ub_1010_1010_0000) 5)
+            (equal (bitscan-fwd #ub_0011_1100_0000) 6))))
 
-(local (defthmd bitscan-fwd-examples
-         ;; This is just to try to "validate the spec" by showing it produces the
-         ;; values we want for some examples.
-         (and
-          ;; Some basic examples...
-          (equal (bitscan-fwd #ub_0000_0000_0001) 0)
-          (equal (bitscan-fwd #ub_0000_0000_0010) 1)
-          (equal (bitscan-fwd #ub_0000_0000_0100) 2)
-          (equal (bitscan-fwd #ub_0000_0000_1000) 3)
-          (equal (bitscan-fwd #ub_0000_0001_0000) 4)
-          (equal (bitscan-fwd #ub_0000_0010_0000) 5)
-          (equal (bitscan-fwd #ub_0000_0100_0000) 6)
-          ;; Same examples, but with upper bits changed to 1s...
-          (equal (bitscan-fwd #ub_0100_0101_0001) 0)
-          (equal (bitscan-fwd #ub_0110_0110_1010) 1)
-          (equal (bitscan-fwd #ub_1010_0101_0100) 2)
-          (equal (bitscan-fwd #ub_1010_1110_1000) 3)
-          (equal (bitscan-fwd #ub_1111_1111_0000) 4)
-          (equal (bitscan-fwd #ub_1010_1010_0000) 5)
-          (equal (bitscan-fwd #ub_0011_1100_0000) 6))))
-
-(defthm natp-of-bitscan-fwd
-  (natp (bitscan-fwd src))
-  :rule-classes :type-prescription)
-
-(defcong nat-equiv equal (bitscan-fwd src) 1
-  :hints(("Goal" :in-theory (enable bitscan-fwd))))
+  (defcong nat-equiv equal (bitscan-fwd src) 1))
 
 
-(defund bitscan-rev (src)
-  "(BITSCAN-REV SRC) returns the bit position of the most significant bit in
-SRC that is set, or 0 when SRC is zero (and hence has no such bit)."
-  (declare (xargs :guard (natp src)
-                  :measure (nfix src)))
+(define bitscan-rev ((src natp))
+  :returns (position natp :rule-classes :type-prescription)
+  :parents (extra-defs)
+  :short "@(call bitscan-rev) returns the bit position of the most significant
+bit in @('src') that is set, or 0 when @('src') is zero (and hence has no such
+bit)."
+  :long "<p>Examples:</p>
+@({
+    (bitscan-rev #b0001) = 0
+    (bitscan-rev #b0011) = 1
+    (bitscan-rev #b0101) = 2
+    (bitscan-rev #b1001) = 3
+})"
+
   (if (zp src)
       0
     (let ((next (ash src -1)))
       (if (= next 0)
           0
-        (+ 1 (bitscan-rev next))))))
+        (+ 1 (bitscan-rev next)))))
+  ///
+  (local (defthmd bitscan-rev-examples
+           ;; This is just to try to "validate the spec" by showing it produces the
+           ;; values we want for some examples.
+           (and
+            ;; Some basic examples... just like bsf since only one bit is set
+            (equal (bitscan-rev #ub_0000_0000_0001) 0)
+            (equal (bitscan-rev #ub_0000_0000_0010) 1)
+            (equal (bitscan-rev #ub_0000_0000_0100) 2)
+            (equal (bitscan-rev #ub_0000_0000_1000) 3)
+            (equal (bitscan-rev #ub_0000_0001_0000) 4)
+            (equal (bitscan-rev #ub_0000_0010_0000) 5)
+            (equal (bitscan-rev #ub_0000_0100_0000) 6)
+            (equal (bitscan-rev #ub_0000_1000_0000) 7)
+            (equal (bitscan-rev #ub_0001_0000_0000) 8)
+            (equal (bitscan-rev #ub_0010_0000_0000) 9)
+            (equal (bitscan-rev #ub_0100_0000_0000) 10)
+            (equal (bitscan-rev #ub_1000_0000_0000) 11)
+            ;; Same examples, but with some low bits flipped to one.
+            (equal (bitscan-rev #ub_0000_0000_0001) 0)
+            (equal (bitscan-rev #ub_0000_0000_0011) 1)
+            (equal (bitscan-rev #ub_0000_0000_0101) 2)
+            (equal (bitscan-rev #ub_0000_0000_1101) 3)
+            (equal (bitscan-rev #ub_0000_0001_0101) 4)
+            (equal (bitscan-rev #ub_0000_0011_0101) 5)
+            (equal (bitscan-rev #ub_0000_0101_0111) 6)
+            (equal (bitscan-rev #ub_0000_1101_1111) 7)
+            (equal (bitscan-rev #ub_0001_1111_1111) 8)
+            (equal (bitscan-rev #ub_0010_0100_0101) 9)
+            (equal (bitscan-rev #ub_0101_0100_0001) 10)
+            (equal (bitscan-rev #ub_1010_0101_0110) 11))))
 
-(defcong nat-equiv equal (bitscan-rev src) 1
-  :hints(("Goal" :in-theory (enable bitscan-rev))))
-
-(local (defthmd bitscan-rev-examples
-         ;; This is just to try to "validate the spec" by showing it produces the
-         ;; values we want for some examples.
-         (and
-          ;; Some basic examples... just like bsf since only one bit is set
-          (equal (bitscan-rev #ub_0000_0000_0001) 0)
-          (equal (bitscan-rev #ub_0000_0000_0010) 1)
-          (equal (bitscan-rev #ub_0000_0000_0100) 2)
-          (equal (bitscan-rev #ub_0000_0000_1000) 3)
-          (equal (bitscan-rev #ub_0000_0001_0000) 4)
-          (equal (bitscan-rev #ub_0000_0010_0000) 5)
-          (equal (bitscan-rev #ub_0000_0100_0000) 6)
-          (equal (bitscan-rev #ub_0000_1000_0000) 7)
-          (equal (bitscan-rev #ub_0001_0000_0000) 8)
-          (equal (bitscan-rev #ub_0010_0000_0000) 9)
-          (equal (bitscan-rev #ub_0100_0000_0000) 10)
-          (equal (bitscan-rev #ub_1000_0000_0000) 11)
-          ;; Same examples, but with some low bits flipped to one.
-          (equal (bitscan-rev #ub_0000_0000_0001) 0)
-          (equal (bitscan-rev #ub_0000_0000_0011) 1)
-          (equal (bitscan-rev #ub_0000_0000_0101) 2)
-          (equal (bitscan-rev #ub_0000_0000_1101) 3)
-          (equal (bitscan-rev #ub_0000_0001_0101) 4)
-          (equal (bitscan-rev #ub_0000_0011_0101) 5)
-          (equal (bitscan-rev #ub_0000_0101_0111) 6)
-          (equal (bitscan-rev #ub_0000_1101_1111) 7)
-          (equal (bitscan-rev #ub_0001_1111_1111) 8)
-          (equal (bitscan-rev #ub_0010_0100_0101) 9)
-          (equal (bitscan-rev #ub_0101_0100_0001) 10)
-          (equal (bitscan-rev #ub_1010_0101_0110) 11))))
-
-(defthm natp-of-bitscan-rev
-  (natp (bitscan-rev src))
-  :rule-classes :type-prescription)
-
-
+  (defcong nat-equiv equal (bitscan-rev src) 1))
 
 
