books/centaur/vl/checkers/dupeinst-check.lisp
@@ -1,5 +1,5 @@
 ; VL Verilog Toolkit
-; Copyright (C) 2008-2011 Centaur Technology
+; Copyright (C) 2008-2013 Centaur Technology
 ;
 ; Contact:
 ;   Centaur Technology Formal Verification Group
@@ -22,6 +22,7 @@
 (include-book "../mlib/expr-tools")
 (include-book "duplicate-detect")
 (local (include-book "../util/arithmetic"))
+
 
 (defxdoc dupeinst-check
   :parents (checkers)
@@ -46,45 +47,46 @@ given to multiple inverters.</p>
 want to identify and eliminate.  For instance, it's especially useful to
 eliminate redundant registers, to improve power usage.</p>")
 
+
 (defaggregate vl-dupeinst-key
-  (modname inputs)
-  :tag :vl-dupeinst-key
-  :require ((vl-exprlist-p-of-vl-dupeinst-key->inputs
-             (vl-exprlist-p inputs))
-            (stringp-of-vl-dupeinst-key->modname
-             (stringp modname)
-             :rule-classes :type-prescription))
   :parents (dupeinst-check)
   :short "Keys used to determine if module instances have the same inputs."
+
+  ((modname stringp :rule-classes :type-prescription
+            "Name of the submodule being instantiated.  We need to know the
+             name of each instance so that we don't get confused by things
+             like
+
+             @({
+                 mymod1 m1 (o1, a, b);
+                 mymod2 m2 (o2, a, b);
+             })
+
+             which, despite having the same arguments, are presumably very
+             different things.")
+
+   (inputs  vl-exprlist-p
+            "Inputs (not outputs or inouts) to the submodule instance.  We
+             expect instances to be argresolved so that these are already in
+             some canonical order.  We just keep the expressions because we
+             don't care about port names, directions, etc.  We also expect all
+             of these expressions to be fixed so that attributes are
+             ignored."))
 
   :long "<p>We generate a key from each modinst.  Modinsts with the same keys
 are regarded as having the same inputs.  That is, the whole point of the
 dupeinst check is to find modinsts with the same key.</p>
 
-<p>The keys we use have to know the modname so we don't get confused by things
-like</p>
-
-@({
-  mymod1 m1 (o1, a, b);
-  mymod2 m2 (o2, a, b);
-})
-
-<p>Which presumably have the same inputs but are very different things.</p>
-
-<p>They also include the expressions for the inputs.  We expect instances to be
-argresolved so that these are already in some canonical order.  We just keep
-the expressions because we don't care about port names, directions, etc.  We
-also expect all of these expressions to be fixed so that attributes are
-ignored.</p>
-
-<p>Our keys should arguably include the params.  But if the inputs are the
-same, then the params should probably be the same or, at any rate, seem
-basically compatible?  Well, whatever.  It's questionable, but probably doesn't
-matter much at all in practice.</p>
+<p>Our keys should arguably include the parameter arguments.  But if the inputs
+are the same, then the parameters should probably be the same or, at any rate,
+seem basically compatible?  Well, whatever.  It probably doesn't matter much at
+all in practice.</p>
 
 <p>We always hons keys because we're going to use them as fast alist keys.</p>"
 
+  :tag :vl-dupeinst-key
   :hons t)
+
 
 (defalist vl-dupeinst-alistp (x)
   :key (vl-dupeinst-key-p x)
@@ -97,90 +99,61 @@ that key, which lets us immediately see which modinsts have the same key.</p>
 @(def vl-dupeinst-alistp)")
 
 
-(defsection vl-make-dupeinst-alist
+(define vl-make-dupeinst-alist-aux
+  ((x     vl-modinstlist-p)
+   (alist vl-dupeinst-alistp))
+  :returns (new-alist vl-dupeinst-alistp :hyp :fguard)
+  :parents (vl-make-dupeinst-alist)
+  (b* (((when (atom x))
+        alist)
+       (x1 (car x))
+       ((vl-modinst x1) x1)
+
+       ((when (vl-arguments->namedp x1.portargs))
+        ;; Args not resolved, skip it
+        (vl-make-dupeinst-alist-aux (cdr x) alist))
+
+       ((mv inputs ?outputs inouts unknowns)
+        (vl-partition-plainargs (vl-arguments->args x1.portargs) nil nil nil nil))
+
+       ((unless (and (atom inouts)
+                     (atom unknowns)))
+        ;; Too hard, skip it
+        (vl-make-dupeinst-alist-aux (cdr x) alist))
+
+       (ins    (vl-plainarglist->exprs inputs))
+       ((when (member nil ins))
+        ;; Blanks?  screw it, skip it.
+        (vl-make-dupeinst-alist-aux (cdr x) alist))
+       (ins    (vl-exprlist-fix ins))
+       (key    (make-vl-dupeinst-key :modname x1.modname :inputs ins))
+       (look   (hons-get key alist))
+       (alist  (hons-acons key (cons x1 (cdr look)) alist)))
+    (vl-make-dupeinst-alist-aux (cdr x) alist)))
+
+(define vl-make-dupeinst-alist ((x vl-modinstlist-p))
+  :returns (alist vl-dupeinst-alistp :hyp :fguard)
   :parents (dupeinst-check)
-  :short "Builds the @(see vl-dupeinst-alistp) for a list of assignments."
+  :short "Builds a (slow) @(see vl-dupeinst-alistp) for a list of assignments."
 
-  (defund vl-make-dupeinst-alist-aux (x alist)
-    (declare (xargs :guard (and (vl-modinstlist-p x)
-                                (vl-dupeinst-alistp alist))))
-    (b* (((when (atom x))
-          alist)
-         (x1 (car x))
-         ((vl-modinst x1) x1)
-
-         ((when (vl-arguments->namedp x1.portargs))
-          ;; Args not resolved, skip it
-          (vl-make-dupeinst-alist-aux (cdr x) alist))
-
-         ((mv inputs ?outputs inouts unknowns)
-          (vl-partition-plainargs (vl-arguments->args x1.portargs) nil nil nil nil))
-
-         ((unless (and (atom inouts)
-                       (atom unknowns)))
-          ;; Too hard, skip it
-          (vl-make-dupeinst-alist-aux (cdr x) alist))
-
-         (ins    (vl-plainarglist->exprs inputs))
-         ((when (member nil ins))
-          ;; Blanks?  screw it, skip it.
-          (vl-make-dupeinst-alist-aux (cdr x) alist))
-         (ins    (vl-exprlist-fix ins))
-         (key    (make-vl-dupeinst-key :modname x1.modname :inputs ins))
-         (look   (hons-get key alist))
-         (alist  (hons-acons key (cons x1 (cdr look)) alist)))
-      (vl-make-dupeinst-alist-aux (cdr x) alist)))
-
-  (local (in-theory (enable vl-make-dupeinst-alist-aux)))
-
-  (defthm vl-dupeinst-alistp-of-vl-make-dupeinst-alist-aux
-    (implies (and (vl-modinstlist-p x)
-                  (vl-dupeinst-alistp alist))
-             (vl-dupeinst-alistp (vl-make-dupeinst-alist-aux x alist))))
-
-  (defund vl-make-dupeinst-alist (x)
-    "Returns a slow alist."
-    (declare (xargs :guard (vl-modinstlist-p x)))
-    (b* ((alist (len x))
-         (alist (vl-make-dupeinst-alist-aux x alist))
-         (ans   (hons-shrink-alist alist nil)))
-      (fast-alist-free alist)
-      (fast-alist-free ans)
-      ans))
-
-  (local (in-theory (enable vl-make-dupeinst-alist)))
-
-  (defthm vl-dupeinst-alistp-of-vl-make-dupeinst-alist
-    (implies (force (vl-modinstlist-p x))
-             (vl-dupeinst-alistp (vl-make-dupeinst-alist x)))))
+  (b* ((alist (len x))
+       (alist (vl-make-dupeinst-alist-aux x alist))
+       (ans   (hons-shrink-alist alist nil)))
+    (fast-alist-free alist)
+    (fast-alist-free ans)
+    ans))
 
 
-
-(defsection vl-maybe-warn-dupeinst
+(defsection vl-dupeinst-trivial-p
   :parents (dupeinst-check)
-  :short "Possibly add warnings about a group of module instances."
-  :long "<p><b>Signature:</b> @(call vl-maybe-warn-dupeinst) returns
-@('warnings'').</p>
+  :short "Customizable filter for duplicate module instances."
 
-<ul>
+  :long "<p>By default, all duplicated modules are considered worth warning
+about.  But you can configure which modules are considered trivial/okay to
+duplicate by attaching a function to @('vl-dupeinst-trivial-p').  These will be
+filtered out into minor warnings.</p>
 
-<li>@('key') is the shared @(see vl-dupeinst-key-p) for a group of
-modinsts.</li>
-
-<li>@('modinsts') are the modinsts that share this key.</li>
-
-<li>@('warnings') is the @(see warnings) accumulator to extend.</li>
-
-</ul>
-
-<p>Modinsts might not have multiple entries, in which case there is nothing to
-do and we just return @('warnings') unchanged.  Otherwise, we issue a warning
-about the modules.</p>
-
-<p>By default, all duplicated modules are considered worth warning about.  But
-you can configure which modules are considered trivial/okay to duplicate by
-attaching a function to @('vl-dupeinst-trivial-p').  These will be filtered out
-into minor warnings.</p>"
+@(def vl-dupeinst-trivial-p)"
 
   (encapsulate
     (((vl-dupeinst-trivial-p *) => *
@@ -197,125 +170,107 @@ into minor warnings.</p>"
              (ignore modname))
     nil)
 
-  (defattach vl-dupeinst-trivial-p vl-dupeinst-trivial-p-default)
-
-  (defun vl-modinstlist-fixed-up-outs (x)
-    (declare (xargs :guard (vl-modinstlist-p x)))
-    (b* (((when (atom x))
-          nil)
-         ((vl-modinst x1) (car x))
-         ((when (vl-arguments->namedp x1.portargs))
-          (er hard? 'vl-modinstlist-fixed-up-outs "expected resolved args"))
-         ((mv ?inputs outputs ?inouts ?unknowns)
-          (vl-partition-plainargs (vl-arguments->args x1.portargs) nil nil nil nil))
-         (outexprs (vl-plainarglist->exprs outputs))
-         (fixed-outexprs (if (member nil outexprs)
-                             ;; Can't fix them up because there are blanks.  Well, who
-                             ;; cares.  We'll just leave them unfixed.
-                             outexprs
-                           (vl-exprlist-fix outexprs))))
-      (cons fixed-outexprs
-            (vl-modinstlist-fixed-up-outs (cdr x)))))
-
-  (defund vl-maybe-warn-dupeinst (key modinsts warnings)
-    "Returns WARNINGS'"
-    (declare (xargs :guard (and (vl-dupeinst-key-p key)
-                                (vl-modinstlist-p modinsts)
-                                (vl-warninglist-p warnings)))
-             (ignorable key))
-    (b* (((when (or (atom modinsts)
-                    (atom (cdr modinsts))))
-          ;; Nothing to do -- there isn't more than one assignment for this RHS.
-          warnings)
-
-         ;; BOZO maybe filter some of this stuff?
-
-         (fixed-up-outs (vl-modinstlist-fixed-up-outs modinsts))
-         (dupes         (duplicated-members fixed-up-outs))
-
-         (modname (vl-dupeinst-key->modname key))
-         (minor-p (vl-dupeinst-trivial-p modname))
-
-         (w (make-vl-warning
-             :type (if (consp dupes)
-                       (if minor-p :vl-warn-same-ports-minor :vl-warn-same-ports)
-                     (if minor-p :vl-warn-same-inputs-minor :vl-warn-same-inputs))
-             :msg "Found instances of the same module with ~s0:~%~%~s1"
-             :args (list (if (consp dupes)
-                             "the same arguments"
-                           "the same inputs (but different outputs)")
-                         (str::prefix-lines (with-local-ps
-                                             ;; may help avoid unnecessary line wrapping
-                                             (vl-ps-update-autowrap-col 200)
-                                             (vl-pp-modinstlist modinsts nil nil))
-                                            "     ")
-                         ;; These aren't printed, but we include them in the
-                         ;; warning so our suppression mechanism can be
-                         ;; applied.
-                         modinsts)
-             :fatalp nil
-             :fn 'vl-maybe-warn-dupeinst)))
-      (cons w warnings)))
-
-  (local (in-theory (enable vl-maybe-warn-dupeinst)))
-
-  (defthm vl-warninglist-p-of-vl-maybe-warn-dupeinst
-    (implies (force (vl-warninglist-p warnings))
-             (vl-warninglist-p (vl-maybe-warn-dupeinst rhs modinsts warnings)))))
+  (defattach vl-dupeinst-trivial-p vl-dupeinst-trivial-p-default))
 
 
-(defsection vl-warnings-for-dupeinst-alist
+
+(define vl-modinstlist-fixed-up-outs ((x vl-modinstlist-p))
+  :parents (vl-maybe-warn-dupeinst)
+  :short "Extract the @(see vl-expr-fix)ed outputs from each module instance."
+  (b* (((when (atom x))
+        nil)
+       ((vl-modinst x1) (car x))
+       ((when (vl-arguments->namedp x1.portargs))
+        (raise "expected resolved args"))
+       ((mv ?inputs outputs ?inouts ?unknowns)
+        (vl-partition-plainargs (vl-arguments->args x1.portargs) nil nil nil nil))
+       (outexprs (vl-plainarglist->exprs outputs))
+       (fixed-outexprs (if (member nil outexprs)
+                           ;; Can't fix them up because there are blanks.
+                           ;; Well, who cares.  We'll just leave them unfixed.
+                           outexprs
+                         (vl-exprlist-fix outexprs))))
+    (cons fixed-outexprs
+          (vl-modinstlist-fixed-up-outs (cdr x)))))
+
+(define vl-maybe-warn-dupeinst
+  ((key      vl-dupeinst-key-p "The shared key for a group of modinsts.")
+   (modinsts vl-modinstlist-p  "The modinsts that share this key.")
+   (warnings vl-warninglist-p  "The @(see warnings) accumulator to extend."))
+  :returns (new-warnings vl-warninglist-p
+                         :hyp (force (vl-warninglist-p warnings)))
   :parents (dupeinst-check)
+  :short "Possibly add warnings about a group of module instances."
+  :long "<p>Modinsts might not have multiple entries, in which case there is
+nothing to do and we just return @('warnings') unchanged.  Otherwise, we issue
+a warning about the modules.</p>"
 
-  (defund vl-warnings-for-dupeinst-alist (alist warnings)
-    (declare (xargs :guard (and (vl-dupeinst-alistp alist)
-                                (vl-warninglist-p warnings))))
-    (b* (((when (atom alist))
-          warnings)
-         (rhs      (caar alist))
-         (assigns  (cdar alist))
-         (warnings (vl-maybe-warn-dupeinst rhs assigns warnings)))
-      (vl-warnings-for-dupeinst-alist (cdr alist) warnings)))
+  (b* (((when (or (atom modinsts)
+                  (atom (cdr modinsts))))
+        ;; Nothing to do -- there isn't more than one assignment for this RHS.
+        warnings)
 
-  (local (in-theory (enable vl-warnings-for-dupeinst-alist)))
+       ;; BOZO maybe filter some of this stuff?
 
-  (defthm vl-warninglist-p-of-vl-warnings-for-dupeinst-alist
-    (implies (force (vl-warninglist-p warnings))
-             (vl-warninglist-p (vl-warnings-for-dupeinst-alist alist warnings)))))
+       (fixed-up-outs (vl-modinstlist-fixed-up-outs modinsts))
+       (dupes         (duplicated-members fixed-up-outs))
+
+       (modname (vl-dupeinst-key->modname key))
+       (minor-p (vl-dupeinst-trivial-p modname))
+
+       (w (make-vl-warning
+           :type (if (consp dupes)
+                     (if minor-p :vl-warn-same-ports-minor :vl-warn-same-ports)
+                   (if minor-p :vl-warn-same-inputs-minor :vl-warn-same-inputs))
+           :msg "Found instances of the same module with ~s0:~%~%~s1"
+           :args (list (if (consp dupes)
+                           "the same arguments"
+                         "the same inputs (but different outputs)")
+                       (str::prefix-lines (with-local-ps
+                                           ;; may help avoid unnecessary line wrapping
+                                           (vl-ps-update-autowrap-col 200)
+                                           (vl-pp-modinstlist modinsts nil nil))
+                                          "     ")
+                       ;; These aren't printed, but we include them in the
+                       ;; warning so our suppression mechanism can be
+                       ;; applied.
+                       modinsts)
+           :fatalp nil
+           :fn 'vl-maybe-warn-dupeinst)))
+    (cons w warnings)))
 
 
-(defsection vl-module-dupeinst-check
+(define vl-warnings-for-dupeinst-alist ((alist    vl-dupeinst-alistp)
+                                        (warnings vl-warninglist-p))
+  :returns (new-warnings vl-warninglist-p
+                         :hyp (force (vl-warninglist-p warnings)))
   :parents (dupeinst-check)
+  (b* (((when (atom alist))
+        warnings)
+       (rhs      (caar alist))
+       (assigns  (cdar alist))
+       (warnings (vl-maybe-warn-dupeinst rhs assigns warnings)))
+    (vl-warnings-for-dupeinst-alist (cdr alist) warnings)))
 
-  (defund vl-module-dupeinst-check (x)
-    (declare (xargs :guard (vl-module-p x)))
-    (b* (((vl-module x) x)
-         (alist    (vl-make-dupeinst-alist x.modinsts))
-         (warnings (vl-warnings-for-dupeinst-alist alist x.warnings)))
-      (change-vl-module x :warnings warnings)))
 
-  (local (in-theory (enable vl-module-dupeinst-check)))
-
-  (defthm vl-module-p-of-vl-module-dupeinst-check
-    (implies (force (vl-module-p x))
-             (vl-module-p (vl-module-dupeinst-check x))))
-
+(define vl-module-dupeinst-check ((x vl-module-p))
+  :parents (dupeinst-check)
+  :returns (new-x vl-module-p :hyp :fguard)
+  (b* (((vl-module x) x)
+       (alist    (vl-make-dupeinst-alist x.modinsts))
+       (warnings (vl-warnings-for-dupeinst-alist alist x.warnings)))
+    (change-vl-module x :warnings warnings))
+  ///
   (defthm vl-module->name-of-vl-module-dupeinst-check
     (equal (vl-module->name (vl-module-dupeinst-check x))
            (vl-module->name x))))
 
-
-(defsection vl-modulelist-dupeinst-check
+(defprojection vl-modulelist-dupeinst-check (x)
+  (vl-module-dupeinst-check x)
+  :guard (vl-modulelist-p x)
+  :result-type vl-modulelist-p
   :parents (dupeinst-check)
-
-  (defprojection vl-modulelist-dupeinst-check (x)
-    (vl-module-dupeinst-check x)
-    :guard (vl-modulelist-p x)
-    :result-type vl-modulelist-p
-    :parents (dupeinst-check))
-
-  (defthm vl-modulelist->names-of-vl-modulelist-dupeinst-check
-    (equal (vl-modulelist->names (vl-modulelist-dupeinst-check x))
-           (vl-modulelist->names x))
-    :hints(("Goal" :induct (len x)))))
+  :rest ((defthm vl-modulelist->names-of-vl-modulelist-dupeinst-check
+           (equal (vl-modulelist->names (vl-modulelist-dupeinst-check x))
+                  (vl-modulelist->names x)))))
 
